aneris/examples/transactional_consistency/implication_trace_util.v
@@ -1,0 +1,297 @@
+From iris.algebra Require Import gset auth gmap excl excl_auth csum.
+From iris.base_logic.lib Require Import mono_nat ghost_map.
+From iris.algebra.lib Require Import mono_list.
+From aneris.algebra Require Import monotone.
+From aneris.aneris_lang Require Import network resources proofmode.
+From aneris.lib Require Import gen_heap_light.
+From aneris.aneris_lang.lib Require Import list_proof inject lock_proof.
+From aneris.aneris_lang.lib.serialization Require Import serialization_proof.
+From aneris.aneris_lang.program_logic Require Import lightweight_atomic.
+From aneris.examples.transactional_consistency Require Import resource_algebras user_params aux_defs state_based_model.
+
+Section trace_proof_util.
+  Context `{!anerisG Mdl Σ, !KVSG Σ, !User_params}.
+
+  Definition trace_inv_name := nroot.@"trinv".
+
+  (** Ghost theory for wrapped resources *)
+
+  (* For the OwnLinTrace/OwnLinHist resources and rules we are reusing trace infrastructure *)
+
+  Definition OwnLinHist (γ : gname) (l : list val) : iProp Σ :=
+    own γ (◯ (gmap_of_trace 0 l)).
+
+  Definition OwnLinTrace (γ : gname) (l : list val) : iProp Σ := 
+    own γ (● gmap_of_trace 0 l) ∗ OwnLinHist γ l.
+
+  Lemma own_lin_hist (γ : gname) (l : list val) :
+    OwnLinTrace γ l ==∗ OwnLinTrace γ l ∗ OwnLinHist γ l.
+  Proof.
+    rewrite /OwnLinTrace.
+    iIntros "(H1 & #H2)".
+    iModIntro.
+    iFrame "#∗".
+  Qed.
+
+  Lemma own_lin_prefix (γ : gname) (l h : list val) :
+    OwnLinTrace γ l ∗ OwnLinHist γ h -∗
+    OwnLinTrace γ l ∗ OwnLinHist γ h ∗ ⌜h `prefix_of` l⌝.
+  Proof.
+    rewrite /OwnLinTrace /OwnLinHist.
+    iIntros "((H1 & H2) & H3)".
+    iDestruct (own_op with "[$H1 $H3]") as "H".
+    iDestruct (own_valid with "H") as %[Hsub Hvalid]%auth_both_valid_discrete.
+    iDestruct "H" as "(H1 & H3)".
+    iFrame.
+    iPureIntro.
+    eapply gmap_of_trace_hist_valid_prefix; eauto.
+  Qed.
+
+  Lemma own_lin_add (γ : gname) (l: list val) (v : val) :
+    OwnLinTrace γ l ==∗ OwnLinTrace γ (l ++ [v]).
+  Proof.
+    rewrite /OwnLinTrace /OwnLinHist.
+    iIntros "(H1 & H2)".
+    rewrite gmap_of_trace_snoc Nat.add_0_l.
+    iMod (own_update_2 with "H1 H2") as "[H1 H2]".
+    apply auth_update.
+    eapply (alloc_local_update _ _ (length l : nat) (to_agree v)); try done.
+    { 
+      eapply not_elem_of_dom.
+      rewrite gmap_of_trace_dom.
+      intro Hfalse. 
+      lia. 
+    }
+    iModIntro. 
+    iFrame.
+  Qed.
+
+  Definition trace_lin_resources (lt t : list val) (γ : gname) : iProp Σ :=
+    ∃ (m : gmap string bool), ⌜∀ (x : string), x ∉ tags t → x ∉ (dom m)⌝ ∗ ghost_map_auth γ (1%Qp) m ∗ 
+      ∀ tag, ⌜(∃ e : val, e ∈ lt ∧ tagOfEvent e = Some tag)⌝ → ghost_map.ghost_map_elem γ tag (DfracOwn 1%Qp) true.
+  
+  Definition trace_post_resources (t : list val) (γ : gname) : iProp Σ :=
+    ∃ (m : gmap string bool), ⌜∀ (x : string), x ∉ tags t → x ∉ (dom m)⌝ ∗ ghost_map_auth γ (1%Qp) m ∗ 
+      ∀ tag, ⌜(∃ e : val, e ∈ t ∧ is_post_event e ∧ tagOfEvent e = Some tag)⌝ → ghost_map.ghost_map_elem γ tag (DfracOwn 1%Qp) true.
+
+  Definition lin_tag_res tag γ := ghost_map.ghost_map_elem γ tag (DfracOwn 1%Qp) true.
+
+  Lemma lin_tag_create lt t γ e tag : 
+    trace_lin_resources lt t γ ∗ ⌜tag ∉ tags t ∧ tagOfEvent e = Some tag ∧ ¬is_post_event e⌝ ==∗
+    trace_lin_resources lt (t ++ [e]) γ ∗ lin_tag_res tag γ.
+  Proof.
+    iIntros "((%m & %Hdom & Hghost_map & Himp) & (%Hnin & %Htag & %Hnot))".
+    assert (m !! tag = None) as Hlookup_none.
+    {
+      apply not_elem_of_dom_1.
+      by apply Hdom.
+    }
+    iMod (ghost_map_insert tag true Hlookup_none with "[$Hghost_map]") as "(Hghost_map & Hkey)".
+    iModIntro.
+    iFrame.
+    iExists (<[tag:=true]> m).
+    iFrame.
+    iPureIntro.
+    intros tag' Hnin'.
+    assert (tag' ∉ tags t) as Hnin''.
+    {
+      specialize (tags_sub e t) as Hsub.
+      set_solver.
+    }
+    specialize (Hdom tag' Hnin'').
+    rewrite dom_insert.
+    assert (tag ∈ tags (t ++ [e])) as Hin.
+    {
+      apply (tags_in e); last done.
+      set_solver.
+    }
+    set_solver.
+  Qed.
+
+  Lemma lin_tag_add lt t γ e tag : 
+    trace_lin_resources lt t γ ∗ lin_tag_res tag γ ∗ ⌜tagOfEvent e = Some tag⌝ -∗
+    trace_lin_resources (lt ++ [e]) t γ.
+  Proof.
+    iIntros "((%m & %Hdom & Hghost_map & Himp) & Hkey & %Htag)".
+    rewrite /trace_lin_resources.
+    iExists m.
+    iFrame.
+    iSplit; first by iPureIntro.
+    iIntros (tag') "%Hpure". 
+    destruct Hpure as (e' & Hin & Htag').
+    rewrite elem_of_app in Hin.
+    destruct Hin as [Hin | Hin].
+    + iApply "Himp".
+      iPureIntro.
+      by exists e'.
+    + assert (e' = e) as ->; first set_solver.
+      assert (tag = tag') as ->; first set_solver.
+      iFrame.
+  Qed.
+
+  Lemma lin_tag_add_post lt t γ e : 
+    trace_lin_resources lt t γ -∗
+    trace_lin_resources lt (t ++ [e]) γ.
+  Proof.
+    iIntros "(%m & %Hdom & Hghost_map & Himp)".
+    rewrite /trace_lin_resources.
+    iExists m.
+    iFrame.
+    iPureIntro.
+    intros tag Hnin.
+    apply Hdom.
+    specialize (tags_sub e t) as Hsub.
+    set_solver.
+  Qed.
+
+  Lemma lin_tag_not_in lt t γ tag : 
+    trace_lin_resources lt t γ ∗ lin_tag_res tag γ -∗ ¬⌜(∃ e : val, e ∈ lt ∧ tagOfEvent e = Some tag)⌝.
+  Proof.
+    iIntros "((%m & %Hdom & Hghost_map & Himp) & Hkey)".
+    iIntros "Hfalse".
+    iDestruct ("Himp" with "[$Hfalse]") as "Hfalse".
+    rewrite /lin_tag_res.
+    iCombine "Hkey" "Hfalse" as "Hfalse".
+    iDestruct (ghost_map_elem_valid with "Hfalse") as "%Hfalse".
+    by rewrite dfrac_valid_own in Hfalse.
+  Qed.
+
+  Definition post_tag_res tag γ := ghost_map.ghost_map_elem γ tag (DfracOwn 1%Qp) true.
+
+  Lemma post_tag_create t γ e tag : 
+    trace_post_resources t γ ∗ ⌜tag ∉ tags t ∧ tagOfEvent e = Some tag ∧ ¬is_post_event e⌝ ==∗
+    trace_post_resources (t ++ [e]) γ ∗ post_tag_res tag γ.
+  Proof.
+    iIntros "((%m & %Hdom & Hghost_map & Himp) & (%Hnin & %Htag & %Hnot))".
+    assert (m !! tag = None) as Hlookup_none.
+    {
+      apply not_elem_of_dom_1.
+      by apply Hdom.
+    }
+    iMod (ghost_map_insert tag true Hlookup_none with "[$Hghost_map]") as "(Hghost_map & Hkey)".
+    iModIntro.
+    iFrame.
+    iExists (<[tag:=true]> m).
+    iFrame.
+    iSplitR.
+    - iPureIntro.
+      intros tag' Hnin'.
+      assert (tag' ∉ tags t) as Hnin''.
+      {
+        specialize (tags_sub e t) as Hsub.
+        set_solver.
+      }
+      specialize (Hdom tag' Hnin'').
+      rewrite dom_insert.
+      assert (tag ∈ tags (t ++ [e])) as Hin.
+      {
+        apply (tags_in e); last done.
+        set_solver.
+      }
+      set_solver.
+    - iIntros (tag') "%Hpure".
+      iApply "Himp".
+      iPureIntro.
+      destruct Hpure as (e' & Hin & Hevent & Htag').
+      exists e'.
+      rewrite elem_of_app in Hin.
+      destruct Hin as [Hin | Hin]; first done.
+      assert (e = e') as ->; set_solver.
+  Qed.
+
+  Lemma post_tag_add t γ e tag : 
+    trace_post_resources t γ ∗ post_tag_res tag γ ∗ ⌜tagOfEvent e = Some tag ∧ is_post_event e⌝ -∗
+    trace_post_resources (t ++ [e]) γ.
+  Proof.
+    iIntros "((%m & %Hdom & Hghost_map & Himp) & Hkey & %Htag)".
+    rewrite /trace_post_resources.
+    iExists m.
+    iFrame.
+    iSplit.
+    - iPureIntro.
+      intros tag' Hin.
+      apply Hdom.
+      specialize(tags_sub e t) as Hsub.
+      set_solver.
+    - iIntros (tag') "%Hpure". 
+      destruct Hpure as (e' & Hin & Htag').
+      rewrite elem_of_app in Hin.
+      destruct Hin as [Hin | Hin].
+      + iApply "Himp".
+        iPureIntro.
+        by exists e'.
+      + assert (e' = e) as ->; first set_solver.
+        assert (tag = tag') as ->; first set_solver.
+        iFrame.
+    Qed.
+
+  Lemma post_tag_not_in t γ tag : 
+    trace_post_resources t γ ∗ post_tag_res tag γ -∗ ¬⌜(∃ e : val, e ∈ t ∧ is_post_event e ∧ tagOfEvent e = Some tag)⌝.
+  Proof.
+    iIntros "((%m & %Hdom & Hghost_map & Himp) & Hkey)".
+    iIntros "Hfalse".
+    iDestruct ("Himp" with "[$Hfalse]") as "Hfalse".
+    rewrite /lin_tag_res.
+    iCombine "Hkey" "Hfalse" as "Hfalse".
+    iDestruct (ghost_map_elem_valid with "Hfalse") as "%Hfalse".
+    by rewrite dfrac_valid_own in Hfalse.
+  Qed.
+
+  (** Predicates for wrapped resources *)
+
+  Definition open_trans (t : transaction) (c : val) (T : list transaction) : Prop :=
+    ∃ op, t ∈ T ∧ last t = Some op ∧ connOfOp op = c ∧ (¬is_cm_op op).
+
+  Definition latest_write (c : val) (k : Key) (ov : option val) (T : list transaction) : Prop := 
+    (ov = None ∧ (∀ t, open_trans t c T → ¬ ∃ v s, (Wr s k v) ∈ t)) ∨
+    (∃ v t tag, ov = Some v ∧ open_trans t c T ∧ (Wr (tag, c) k v) ∈ t ∧
+      (∀ op, op ∈ t → (∃ s' v', op = Wr s' k v' ∧ op ≠ Wr (tag, c) k v) → rel_list t op (Wr (tag, c) k v))).
+
+  Definition tag_eq (e1 e2 : val) : Prop := ∃ tag, tagOfEvent e1 = Some tag ∧ tagOfEvent e2 = Some tag.
+
+  Definition no_emit_with_address (sa : socket_address) (ltrace : list val) (extract : val → option val)  : Prop := 
+    ¬∃ e c, e ∈ ltrace ∧ connOfEvent e = Some c ∧ extract c = Some #sa.
+
+  Definition active_trace_resources lt T s c γ (m : gmap Key (option val)) : iProp Σ :=
+    ∃ domain sub_domain tail, ⌜s = Active domain⌝ ∗ 
+      ⌜sub_domain = domain ∩ KVS_keys⌝ ∗ ⌜open_start c lt tail⌝ ∗ 
+      ([∗ set] k ∈ KVS_keys ∖ sub_domain, ∃ ov, ghost_map_elem γ k (DfracOwn 1%Qp) ov) ∗ 
+      (∀ k, ⌜k ∈ sub_domain⌝ → ∀ ov, ⌜m !! k = Some ov⌝ → ⌜latest_write c k ov T⌝).
+
+  Definition inactive_trace_resources lt T s c γ : iProp Σ :=
+    ⌜s = CanStart⌝ ∗ ⌜commit_closed c lt⌝ ∗ ⌜¬∃ t, open_trans t c T⌝ ∗
+    ([∗ set] k ∈ KVS_keys, ∃ ov, ghost_map_elem γ k (DfracOwn 1%Qp) ov).
+
+  Definition initialized_trace_resources lt T sa γmname (extract : val → option val)
+  (mstate : gmap socket_address (local_state * option val)) : iProp Σ :=
+    ∃ s c γ (m : gmap Key (option val)), ⌜mstate !! sa = Some (s, Some c)⌝ ∗
+      ⌜extract c = Some #(LitSocketAddress sa)⌝ ∗ 
+      ghost_map_elem γmname sa DfracDiscarded (γ, c) ∗ 
+      ghost_map_auth γ (1%Qp) m ∗ 
+      ⌜(∃ e, e ∈ lt ∧ connOfEvent e = Some c ∧ is_in_lin_event e)⌝ ∗ 
+      (inactive_trace_resources lt T s c γ ∨ active_trace_resources lt T s c γ m).
+
+  Definition unnitialized_trace_resources sa (mstate : gmap socket_address (local_state * option val)) 
+  (mname : gmap socket_address (gname * val)) lt (extract : val → option val) : Prop := 
+    (mstate !! sa = None ∨ mstate !! sa = Some (CanStart, None)) ∧ 
+    (¬∃ p, mname !! sa = Some p) ∧ no_emit_with_address sa lt extract.
+
+  Definition client_trace_state_resources (lt : list val) (T : list transaction) (sa : socket_address) 
+  (γmstate γmname : gname) (extract : val → option val)  (mstate : gmap socket_address (local_state * option val)) 
+  (mname : gmap socket_address (gname * val)) : iProp Σ := 
+    ⌜unnitialized_trace_resources sa mstate mname lt extract⌝ ∨ initialized_trace_resources lt T sa γmname extract mstate.
+
+  Definition trace_state_resources (lt : list val) (T : list transaction) (γmstate γmname : gname) 
+  (clients : gset socket_address) (extract : val → option val) : iProp Σ := 
+    ∃ (mstate : gmap socket_address (local_state * option val)), ghost_map_auth γmstate (1%Qp) mstate ∗ 
+      ∃ (mname : gmap socket_address (gname * val)), ghost_map_auth γmname (1%Qp) mname ∗ 
+        ([∗ set] sa ∈ clients, client_trace_state_resources lt T sa γmstate γmname extract mstate mname).
+
+  Definition GlobalInvExt (extract : val → option val) (γmstate γmlin γmpost γmname γl : gname) (clients : gset socket_address) : iProp Σ := 
+    ∃ t lt T, trace_is t ∗ OwnLinTrace γl lt ∗ ⌜lin_trace_of lt t⌝ ∗ ⌜∀ t, t ∈ T → t ≠ []⌝ ∗
+      ⌜extraction_of lt T⌝ ∗ ⌜valid_transactions T⌝ ∗ ⌜valid_sequence lt⌝ ∗
+      trace_state_resources lt T γmstate γmname clients extract ∗
+      trace_lin_resources lt t γmlin ∗
+      trace_post_resources t γmpost.
+
+End trace_proof_util.
